{
 "cells": [
  {
   "cell_type": "markdown",
   "metadata": {},
   "source": [
    "# Limit and Continuity"
   ]
  },
  {
   "cell_type": "markdown",
   "metadata": {},
   "source": [
    "Let $f, g$ be functions $\\mathbb R^n \\rightarrow \\mathbb R$\n",
    "\n",
    "__Claim 1.__ If $f$ is continuous and $g$ is discontinuous at $a\\in \\mathbb R^n$, then $f+g$ must be discontinuous at $a$. \n",
    "\n",
    "_proof_. Assume $f$ is continuous and $g$ is discontinuous at $a\\in \\mathbb R^n$.  \n",
    "Let $L\\in\\mathbb R$ be arbitrary.  \n",
    "By the definition of discontinuity, take $\\epsilon_g > 0$ s.t. $\\forall \\delta > 0. \\exists x\\in \\mathbb R^n. |x-a|<\\delta \\land |g(x) -g(a)| \\geq \\epsilon_g$.  \n",
    "By the definition of continuity, take $\\delta_f > 0$ s.t. $\\forall x\\in \\mathbb R^n. |x-a| < \\delta_f\\Rightarrow |f(x) -f(a)| < \\epsilon_g/2$  \n",
    "Then, take $\\epsilon = \\epsilon_g/2$. Let $\\delta > 0$ be arbitrary. Take $x\\in\\mathbb R^n. |x-a| < \\min(\\delta, \\delta_f)$.  Therefore, \n",
    "\\begin{align*}\n",
    "\\|f(x) - f(a) + g(x) - g(a)\\| &= \\|(f(x) - f(a)) - (g(a) - g(x))\\|  \\\\\n",
    "&\\geq \\big\\|\\|f(x) - f(a)\\| - \\|g(a) - g(x)\\|\\big\\| &\\text{reverse triangle ineq.}\\\\\n",
    "&\\geq \\epsilon_g/2\\\\\n",
    "&= \\epsilon\n",
    "\\end{align*}\n",
    "Therefore, we prove that \n",
    "$$\\forall L\\in \\mathbb R. \\exists \\epsilon > 0, \\forall \\delta > 0. \\exists x\\in \\mathbb R^n. \\|x-a\\|<\\delta \\land \\|f(x)+g(x)-(f(a)+g(a))\\| \\geq \\epsilon$$"
   ]
  },
  {
   "cell_type": "markdown",
   "metadata": {},
   "source": [
    "__Claim 2.__ If both $f, g$ are discontinuous at $a\\in \\mathbb R^n$, then $f+g$ can be either continuous or discontinuous.   \n",
    "\n",
    "_proof_. Consider the following examples,   \n",
    "Take $f_1(x) := \\begin{cases}1 &x = a\\\\0&x\\neq a\\end{cases}$ and $g_1(x):= \\begin{cases}-1 &x = a\\\\0&x\\neq a\\end{cases}$. Obviously $f_1+g_1$ is continuous at $a$.  \n",
    "Take $f_2(x) := \\begin{cases}1 &x = a\\\\0&x\\neq a\\end{cases}$ and $g_2(x):= \\begin{cases}1 &x = a\\\\0&x\\neq a\\end{cases}$. Obviously $f_2+g_2$ is discontinuous at $a$. "
   ]
  },
  {
   "cell_type": "markdown",
   "metadata": {},
   "source": [
    "__Claim 3.__ If $f$ is continuous and $g$ is discontinuous at $a\\in \\mathbb R^n$, then $f\\times g$ can be either continuous or discontinuous.   \n",
    "\n",
    "_proof_. Consider the following examples,   \n",
    "\n",
    "One of $f, g$ is continuous:  \n",
    "Take $f_1(x) := 0$ and $g_1(x):= \\begin{cases}1 &x = a\\\\0&x\\neq a\\end{cases}$. $f_1(x) g_1(x) = 0$ is continuous at $a$.   \n",
    "Take $f_2(x) := 1$ and $g_2(x):= \\begin{cases}1 &x = a\\\\0&x\\neq a\\end{cases}$. $f_2(x)g_2(x) = g_2(x)$ is discontinuous at $a$. \n",
    " \n",
    "Both $f$ and $g$ are discontinuous:  \n",
    "Take $f_3(x) := \\begin{cases}1 &x = a\\\\0&x\\neq a\\end{cases}$ and $g_3(x):= \\begin{cases}0 &x = a\\\\1&x\\neq a\\end{cases}$. Obviously $f_1(x)g_1(x) = 0$ is continuous at $a$.   \n",
    "Take $f_4(x) := \\begin{cases}1 &x = a\\\\0&x\\neq a\\end{cases}$ and $g_4(x):= \\begin{cases}1 &x = a\\\\0&x\\neq a\\end{cases}$. Obviously $f_4(x)g_4(x) = f_4(x)$ is continuous at $a$.  "
   ]
  },
  {
   "cell_type": "markdown",
   "metadata": {},
   "source": [
    "__Claim.__ if $f:\\mathbb R^n\\rightarrow \\mathbb R$ is continuous, then $S = \\{x\\in\\mathbb R^n:f(x)>0\\}$ is open.\n",
    "\n",
    "_proof_. Let $f:\\mathbb R^n\\rightarrow \\mathbb R$ be continuous.  \n",
    "Let $x_0\\in\\mathbb R^n$ be arbitrary, assume $f(x_0) = L > 0$.  \n",
    "By continuity of $f$, take $\\delta > 0$ s.t. $\\forall x\\in\\mathbb R^n. |x-x_0| < \\delta \\Rightarrow |f(x) - f(x_0)| < L/2$.  \n",
    "Then, note that $|f(x) - f(x_0)| < L/2 \\Rightarrow f(x) > f(x_0) - L/2 = L/2 > 0$.   \n",
    "This implies that $\\forall x \\in B(\\delta, x_0). x\\in S$.  \n",
    "Therefore, we have shown that $\\forall x_0 \\in S. \\exists \\delta > 0. s.t. B(\\delta, x_0) \\subset S$, which means $S$ is open. "
   ]
  },
  {
   "cell_type": "markdown",
   "metadata": {},
   "source": [
    "Find $a$ s.t. $\\forall \\delta > 0, \\exists x \\in S. 0 < |x-a| < \\delta$\n",
    "\n",
    "__(1)__ $S = \\{(x, y)\\in\\mathbb R^2. x^2 +y^2 < 1\\}\\cup\\{(0, 2)\\}$. \n",
    "\n",
    "__Claim__ $\\forall a\\in \\{(x, y)\\in\\mathbb R^2. x^2 +y^2 < 1\\}$, the condition is satisfied. \n",
    "\n",
    "_proof_. Let $a = (x_0, y_0)$ s.t. $x_0^2 + y_0^2 = c < 1$ be arbitrary.  Take $\\epsilon_0 = 1-c, 0 < \\epsilon_0 < 1$.  \n",
    "Let $\\delta > 0$ be arbitrary.  \n",
    "Take $\\epsilon = \\min(\\frac{\\epsilon_0}4, \\frac{\\epsilon_0}{4|x_0 + y_0|}, \\frac{\\delta}2)$, then note that \n",
    "$$|2\\epsilon(x_0 + y_0)| \\leq 2\\frac{\\epsilon_0}{4|x_0+y_0|}|x_0+y_0| \\leq \\epsilon_0/2$$\n",
    "$$2\\epsilon^2 \\leq 2\\frac{\\epsilon_0^2}{4^2} = \\epsilon_0^2/8$$\n",
    "so that \n",
    "\\begin{align*}\n",
    "(x_0 + \\epsilon)^2 + (y_0 + \\epsilon)^2 &\\leq x^2_0 + y^2_0  + |2\\epsilon (x_0 + y_0)| + 2\\epsilon^2\\\\\n",
    "&\\leq x_0^2 + y_0^2 + \\epsilon_0/2 + \\epsilon_0^2/8\\\\\n",
    "&\\leq x_0^2 + y_0^2 + \\epsilon_0/2 + \\epsilon_0/8 &0<\\epsilon_0<1\\\\\n",
    "&< x_0^2 + y_0^2 + \\epsilon_0\\\\\n",
    "&= c + 1 - c \\\\\n",
    "& = 1\\\\\n",
    "&\\Rightarrow (x_0 + \\epsilon, y_0 + \\epsilon) \\in S\n",
    "\\end{align*}\n",
    "Also, \n",
    "$$|(x_0, y_0) - (x_0 + \\epsilon, y_0 + \\epsilon)| = \\sqrt 2\\epsilon \\leq \\sqrt 2\\frac{\\delta}2 = \\delta/\\sqrt 2 < \\delta$$\n",
    "Therefore, $\\forall a\\in S_1. \\forall \\delta > 0, \\exists x\\in S. |x-a| < \\delta$\n",
    "\n",
    "__Claim__. $a = (0, 2)$ does not satisfy the condition. \n",
    "\n",
    "_proof_. Let $(x_0, y_0)\\in S - \\{(0, 2)\\} = \\{(x, y)\\in\\mathbb R^2: x^2 +y^2 < 1\\}$. \n",
    "Note that $0 < x_0^2 + y_0^2 < 1$, so that $-\\sqrt1 < y_0 < \\sqrt 1$.  \n",
    "Therefore, $(y_0-2)^2 > (1-2)^2 = 1$\n",
    "\n",
    "\\begin{align*}\n",
    "|(x_0, y_0) - (0, 2)| &= \\sqrt{(x_0-0)^2 + (y_0-2)^2} \\\\\n",
    "&\\geq \\sqrt{(y_0-2)^2}\\\\\n",
    "&\\geq 1\n",
    "\\end{align*}\n",
    "Therefore, $\\forall x\\in S. |x-(0, 2)| \\leq 0 \\lor |x-(0, 2)|\\geq 1$"
   ]
  },
  {
   "cell_type": "markdown",
   "metadata": {},
   "source": [
    "__(2)__ $S = \\{(x, y)\\in\\mathbb R^2. x^2 +y^2 < 1\\}\\cup\\{(0, 1)\\}$.\n",
    "\n",
    "__Claim.__ $\\forall a\\in S$, the condition is satisfied.   \n",
    "\n",
    "\n",
    "_proof._ We only need to show that \n",
    "$$\\forall \\delta > 0. \\exists x\\in S. 0 < |x-(0, 1)| < \\delta$$\n",
    "The rest are proven in (1). \n",
    "\n",
    "Let $\\delta > 0$. Take $\\delta_0 = \\min(0.1, \\delta/2)$.  \n",
    "Then, \n",
    "$$|(0, 1-\\delta_0) - (0, 1)| = 1-\\delta_0 - 1 = \\delta_0$$\n",
    "Note that $\\delta_0 \\leq 2/\\delta < \\delta$ and $0 + (1-\\delta_0)^2 = 1 - 2\\delta_0 + \\delta_0^2 \\leq 1 - 0.2 + 0.01 < 1$\n",
    "Therefore, $(0, 1-\\delta_0)\\in S$ and $0 < |(0, 1-\\delta_0) - (0, 1)| < \\delta$. "
   ]
  },
  {
   "cell_type": "markdown",
   "metadata": {},
   "source": [
    "__(3)__ $S = \\{(0, 2^{-n})\\in\\mathbb R^2:n\\in\\mathbb N\\}$\n",
    "\n",
    "__Claim.__ $\\forall a\\in S$, the condition does NOT satisfy. \n",
    "\n",
    "_proof_. Let $a = (0, 2^{-n})\\in S$ for some $n\\in\\mathbb N$.  \n",
    "Take $\\delta = 2^{-(n+1)} > 0$.  \n",
    "Then, let $m\\in\\mathbb N, m\\neq n$. \n",
    "$$|(0, 2^{-n}) - (0, 2^{-m})| = |2^{-n}- 2^{-m}| = 2^{-n}|1-2^{n-m}|$$\n",
    "Suppose $m > n$, then $2^{n-m} \\leq 2^{-1}, |1-2^{n-m}|\\geq 1/2$.  \n",
    "Suppose $n > m$, then $2^{n-m} \\geq 2, |1-2^{n-m}| \\geq 1$. \n",
    "\n",
    "Therefore, $|(0, 2^{-n}) - (0, 2^{-m})| \\geq 2^{-n}/2 = 2^{-(n+1)}$"
   ]
  },
  {
   "cell_type": "markdown",
   "metadata": {},
   "source": [
    "__(4)__ $S = \\{(0, 2^{-n})\\in\\mathbb R^2:n\\in \\mathbb N\\}\\cup \\{(0, 0)\\}$\n",
    "\n",
    "__Claim.__ $a = (0, 0)$ satisfies the condition\n",
    "\n",
    "_proof_. For any $\\delta > 0$, we can find some $n\\in\\mathbb N$ s.t. $2^{-n} < \\delta$ so that $0 < |(0, 2^{-n}) - (0, 0)| = 2^{-n} < \\delta$\n",
    "\n",
    "__Claim.__ $\\forall a\\in \\{(0, 2^{-n})\\in\\mathbb R^2. n\\in\\mathbb N\\}, a$ does not satisfy the condition. \n",
    "\n",
    "_proof_. In addition to points in (3), further notice that \n",
    "$\\forall n\\in\\mathbb N$. $|(0, 2^{-n}) - (0, 0)| = 2^{-n} > 2^{-(n+1)}$"
   ]
  },
  {
   "cell_type": "markdown",
   "metadata": {},
   "source": [
    "__Claim.__ For $f:\\mathbb R^n\\rightarrow \\mathbb R^k$ and $g: \\mathbb R^k\\rightarrow\\mathbb R^l$, if $f$ is continuous at $a\\in\\mathbb R^n$ and $g$ is continuous at $f(a)$, then $g\\circ f$ is continuous at $a$. \n",
    "\n",
    "_proof_. Let $\\epsilon > 0$.  \n",
    "Because $g$ is continuous at $f(a)$, take $\\delta_1 > 0$ s.t. $\\forall y\\in\\mathbb R^k. |y-f(a)| < \\delta_1 \\Rightarrow |g(y) - g(f(a))| < \\epsilon$.  \n",
    "Because $f$ is continuous at $a$, take $\\delta_2 > 0$ s.t. $\\forall x\\in\\mathbb R^n. |x - a|  < \\delta_2 \\Rightarrow |f(x) - f(a)| < \\delta_1$  \n",
    "Therefore, for any $x\\in\\mathbb R^n. |x-a| <\\delta_2\\Rightarrow |f(x) - f(a)| < \\delta_1\\Rightarrow |g(f(x)) - g(f(a))| < \\epsilon$. "
   ]
  },
  {
   "cell_type": "markdown",
   "metadata": {},
   "source": [
    "# Sequences and completeness"
   ]
  },
  {
   "cell_type": "markdown",
   "metadata": {},
   "source": [
    "\n",
    "__Claim__. $\\vec a_j\\rightarrow \\vec a \\land \\vec b_j\\rightarrow \\vec b\\Rightarrow \\vec a_j\\cdot \\vec b_j \\rightarrow \\vec a \\cdot \\vec b$\n",
    "\n",
    "_proof_. First note that $\\vec a_j \\rightarrow \\vec a\\Rightarrow \\forall i\\in \\{1, 2, ..., n\\}. a_{ij}\\rightarrow a_{i\\cdot}, b_{ij}\\rightarrow b_{i\\cdot}$, where $a_{ij}$ is the $i$th component of $\\vec a_j$ and $a_{i\\cdot}$ is the $i$th component of $\\vec a$. Then, note that \n",
    "$$\\vec a_j\\cdot \\vec b_j = \\sum_{i=1}^n a_{ij}b_{ij}$$\n",
    "Therefore, apply limit laws for addition and multiplication for 1-D case, \n",
    "$$\\lim_{j\\rightarrow\\infty}\\sum_{i=1}^n a_{ij}b_{ij} = \\sum_{i=1}^n a_{i\\cdot}b_{i\\cdot} = \\vec a\\cdot \\vec b$$"
   ]
  },
  {
   "cell_type": "markdown",
   "metadata": {},
   "source": [
    "__Claim__. For $\\{a_j\\}_j\\subset \\mathbb R^n$ and function $f:\\mathbb R^n\\rightarrow\\mathbb R^k$. If $a_j\\rightarrow a$ and $f$ continuous and $a$, then $f(a_j)\\rightarrow f(a)$. \n",
    "\n",
    "_proof_. Let $\\epsilon > 0$ be arbitrary.  \n",
    "Since $f$ is continuous at $a$, take $\\delta > 0$ s.t. $\\forall x\\in\\mathbb R^n. |x-a|<\\delta\\Rightarrow |f(x)-f(a)| < \\epsilon$.   \n",
    "Since $a_j\\rightarrow a$, take $N\\in\\mathbb N^+$ s.t. $\\forall n \\in\\mathbb N^+. n > N\\Rightarrow |a_n - a| < \\delta$.  \n",
    "Therefore, $|a_n - a| < \\delta \\Rightarrow |f(a_n) - f(a)| < \\epsilon$.  \n",
    "We have proven that $\\forall \\epsilon > 0. \\exists N\\in\\mathbb N^+. \\forall n \\in\\mathbb N^+ . n > N \\Rightarrow |f(a_n) - f(a)| < \\epsilon$. By definition of convergence, $\\lim_{j\\rightarrow \\infty}f(a_j) = f(a)$"
   ]
  },
  {
   "cell_type": "markdown",
   "metadata": {},
   "source": [
    "# Compactness and applications"
   ]
  },
  {
   "cell_type": "markdown",
   "metadata": {},
   "source": [
    "__Claim__ If $S \\subseteq \\mathbb R^n$ is closed and $\\{x_j\\}_j \\subseteq\\mathbb R^n$ converges to $x\\not\\in S$, then $\\exists j\\in\\mathbb N^+. x_j\\not\\in S$. \n",
    "\n",
    "_proof_. First, note that $x\\not\\in S\\Rightarrow x\\in S^c$ and $S$ is closed $\\Rightarrow S^c$ is open.  \n",
    "By the definition of open set, take $\\epsilon > 0$ s.t. $B(\\epsilon, x) \\subset S^c$.  \n",
    "Then, note that $x_j\\rightarrow x$, by the definition of convergent sequence, take $N\\in\\mathbb N^+$ s.t. $\\forall n \\in\\mathbb N^+. n \\geq N\\Rightarrow |x_n - x| < \\epsilon$.  \n",
    "Therefore, note that $|x_N - x|< \\epsilon \\Rightarrow x_N \\in B(\\epsilon, x) \\subset S^c\\Rightarrow x_N\\not\\in S$"
   ]
  },
  {
   "cell_type": "markdown",
   "metadata": {},
   "source": [
    "__Claim.__ If $S$ is unbounded, then exists some $\\{x_j\\}_j\\subset S$ that has no convergent subsequence. \n",
    "\n",
    "_proof_. Construct $\\{x_j\\}_j$ by the following recursive procedure.  \n",
    "Let $x_1\\in S, x_1\\neq 0$ be arbitrary, let $r_1 = \\|x_1\\|$.  \n",
    "Given $x_n, r_n$, let $x_{n+1} \\in S - B(2r_n, 0), r_{n+1} = \\|x_{n+1}\\|$.  \n",
    "Note that such $x_{n+1}$ always exists since $S$ is unbounded.   \n",
    "Also, note that $r_{n+1} = \\|x_{n+1}\\| \\geq 2r_n \\geq 2^{n-1} r_1$. \n",
    "\n",
    "\n",
    "Then, we will show such sequence has no convergent subsequence.   \n",
    "Given any subsequence $\\{x_{k_j}\\}_j$,  \n",
    "Let $L\\in S$ be arbitrary, let $J > 0$ be arbitrary.  \n",
    "Take some $j \\geq J$ s.t. $2^{k_j-1}r_1  \\geq 1 + \\|L\\|$, since $r_1 > 0$ we can always find such $j$.   \n",
    "Therefore, \n",
    "\\begin{align*}\n",
    "\\|x_{k_j} - L\\| &\\geq \\big\\| \\|x_{k_j}\\| - \\|L\\|\\big\\| &\\text{reverse triangle ineq.} \\\\\n",
    "&= 2^{k_j-1}r_1 - \\|L\\| \\\\\n",
    "&\\geq 1 + \\|L\\| - \\|L\\|\\\\\n",
    "& = 1\n",
    "\\end{align*}\n",
    "Therefore, $\\{x_{k_j}\\}_j$ diverges. "
   ]
  },
  {
   "cell_type": "markdown",
   "metadata": {},
   "source": [
    "__lemma__ Any subsequence of convergent sequence will also converge to the same limit.  \n",
    "\n",
    "_proof_. Let $\\{a_j\\}_j$ be convergent to some $L$. Let $\\{a_{k_j}\\}_j$ be some subsequence.    \n",
    "Let $\\epsilon > 0$ be arbitrary, take $J\\in\\mathbb N^+$ s.t. $\\forall j > J. \\|a_j-L\\| < \\epsilon$.  \n",
    "Take $J_2 \\in \\mathbb N^+$ s.t. $k_{J_2} \\geq J$ so that $\\forall j > J_2. k_j > k_{J_2} \\geq J$.  \n",
    "Therefore, $\\forall j > J_2. \\|a_{k_j}- L\\| < \\epsilon$. \n",
    "\n",
    "\n",
    "__Claim.__ The Cartesian Product of two compact sets is compact. \n",
    "\n",
    "_proof_. Let $K_1 \\subseteq \\mathbb R^n, K_2 \\subseteq \\mathbb R^m$  be compact.  \n",
    "Let $\\{(x_j, y_j)\\}_j$ be a sequence in $K_1\\times K_2$ so that $\\{x_j\\}_j\\in K_1, \\{y_j\\}_j \\in K_2$.  \n",
    "By compactness of $K_1$, take subsequence $\\{x_{k_j}\\}_j$ that converge to some $L_1\\in K_1$.  \n",
    "By compactness of $K_2$, further take $\\{y_{l_{k_j}}\\}_j$ be a subsequence of $\\{y_{k_j}\\}_j$ that converge to some $L_2\\in K_2$.  \n",
    "Then, since $\\{x_{l_{k_j}}\\}_j$ is a subsequence of $\\{x_{k_j}\\}_j$, $\\{x_{l_{k_j}}\\}_j$ will also converge to $L_1$ (using lemma above).  \n",
    "Therefore, $\\{(x_{l_{k_j}}, y_{l_{k_j}})\\}_{j}\\rightarrow (L_1, L_2) \\in K_1\\times K_2$  \n",
    "By definition of compactness, $K_1\\times K_2$ is compact. "
   ]
  },
  {
   "cell_type": "markdown",
   "metadata": {},
   "source": [
    "__Claim.__ The closed subset of a compact set is compact.  \n",
    "\n",
    "_proof 1._  If $S$ is compact, then by BW theorem $S$ is closed and bounded. so that $\\forall s\\in S. s\\in B(R, 0)$ for some $R > 0$. Then, for any closed subset $A \\subseteq S$, $s\\in A\\Rightarrow s\\in S\\Rightarrow s\\in B(R, 0)$ so that $A$ is also bounded. Therefore, $A$ is also closed and bounded, hence compact. "
   ]
  },
  {
   "cell_type": "markdown",
   "metadata": {},
   "source": [
    "# Chain Rule\n",
    "\n",
    "\n",
    "__Claim.__ $q(x): = |x|^2. \\nabla q(x) = 2x$\n",
    "\n",
    "_proof_ For any $x\\in\\mathbb R^n$, \n",
    "\\begin{align*}\n",
    "\\lim_{h\\rightarrow 0} \\frac{q(x+h) - q(x) - 2x\\cdot h}{|h|} &= \\lim_{h\\rightarrow 0} \\frac{|x+h|^2 - |x|^2 - 2x\\cdot h}{|h|}\\\\\n",
    "&= \\lim_{h\\rightarrow 0}\\frac{|x|^2 + 2x\\cdot h + |h|^2 -|x|^2-2x\\cdot h}{|h|}\\\\\n",
    "&= \\lim_{h\\rightarrow 0} \\frac{|h|^2}{|h|}\\\\\n",
    "&= \\lim_{h\\rightarrow} h\\\\\n",
    "&= 0\n",
    "\\end{align*}\n",
    "Therefore, by the definition of derivative $\\nabla q = 2x$"
   ]
  },
  {
   "cell_type": "markdown",
   "metadata": {},
   "source": [
    "__Proposition__ Prove chain rule for $g: \\mathbb R\\rightarrow \\mathbb R^2, f: \\mathbb R^2 \\rightarrow \\mathbb R. \\phi = f\\circ g$\n",
    "\n",
    "Given that \n",
    "\\begin{align*}\n",
    "\\phi(t+h) - \\phi(t) = &[f(x(t+h), y(t+h)) - f(x(t+h), y(t))] &(i)\\\\\n",
    "&\\quad+ [f(x(t+h), y(t)) - f(x(t), y(t))] &(ii)\n",
    "\\end{align*}\n",
    "\n",
    "First, write $g(x)=f(x, y)$ so that\n",
    "\\begin{align*}\n",
    "(i) &= g(x(t+h)) - f(x(t)) \\\\\n",
    "&= (x(t+h) - x(t))g'(x(t)+\\theta_{11}(x(t+h) - x(t)))\\\\\n",
    "&= h(x'(t+\\theta_{12}h))g'(x(t)+\\theta_{11}(x(t+h) - x(t)))\\\\\n",
    "&= h\\frac{\\partial x}{\\partial t}(t+\\theta_{12}h)\\frac{\\partial f}{\\partial x}(x(t) - \\theta_{11}(x(t+h) - x(t)))\n",
    "\\end{align*}\n",
    "by MVT, where $\\theta_{11}, \\theta_{12}\\in (0, 1)$.\n",
    "Similarly, \n",
    "$$(ii) = h\\frac{\\partial y}{\\partial t}(t+\\theta_{22}h)\\frac{\\partial f}{\\partial y}(y(t) - \\theta_{21}(y(t+h) - y(t)))$$\n",
    "\n",
    "Therefore, \n",
    "\\begin{align*}\n",
    "\\phi'(t) &= \\lim_{h\\rightarrow 0} h^{-1} \\phi(t+h) - \\phi(t)\\\\\n",
    "&= \\lim_{h\\rightarrow 0} h^{-1}\\\\\n",
    "&\\quad\\bigg[h\\frac{\\partial x}{\\partial t}(t+\\theta_{12}h)\\frac{\\partial f}{\\partial x}(x(t) - \\theta_{11}(x(t+h) - x(t))) \\\\\n",
    "& \\quad + h\\frac{\\partial y}{\\partial t}(t+\\theta_{22}h)\\frac{\\partial f}{\\partial y}(y(t) - \\theta_{21}(y(t+h) - y(t)))\\bigg]\\\\\n",
    "&= \\lim_{h\\rightarrow 0} \\\\\n",
    "&\\quad\\bigg[\\frac{\\partial x}{\\partial t}(t+\\theta_{12}h)\\frac{\\partial f}{\\partial x}(x(t) - \\theta_{11}(x(t+h) - x(t))) \\\\\n",
    "& \\quad + \\frac{\\partial y}{\\partial t}(t+\\theta_{22}h)\\frac{\\partial f}{\\partial y}(y(t) - \\theta_{21}(y(t+h) - y(t)))\\bigg] &(*)\n",
    "\\end{align*}\n",
    "Then, by our assumption, $x, y$ are differentiable, hence continuous, by continuous mapping theorem, \n",
    "$$\\lim_{h\\rightarrow 0} x(t+h) = x(t). \\lim_{h\\rightarrow 0} y(t+h) = y(t)$$\n",
    "In addition, $\\theta_{11}, \\theta_{12}, \\theta_{21}, \\theta_{22}\\in (0, 1)$. Therefore, the limit above exists and equals to\n",
    "$$(*) = \\frac{\\partial x}{\\partial t}(t)\\frac{\\partial f}{\\partial x}(x(t)) + \\frac{\\partial y}{\\partial t}(t)\\frac{\\partial f}{\\partial y}(y(t)) = \\frac{\\partial f}{\\partial x}\\frac{\\partial x}{\\partial t} + \\frac{\\partial f}{\\partial y}\\frac{\\partial y}{\\partial t}$$"
   ]
  }
 ],
 "metadata": {
  "hide_input": false,
  "kernelspec": {
   "display_name": "Python 3",
   "language": "python",
   "name": "python3"
  },
  "language_info": {
   "codemirror_mode": {
    "name": "ipython",
    "version": 3
   },
   "file_extension": ".py",
   "mimetype": "text/x-python",
   "name": "python",
   "nbconvert_exporter": "python",
   "pygments_lexer": "ipython3",
   "version": "3.7.6"
  }
 },
 "nbformat": 4,
 "nbformat_minor": 4
}
