{
 "cells": [
  {
   "cell_type": "raw",
   "metadata": {},
   "source": [
    "---\n",
    "title: Constrainted Optimization on Calulus of Variations Additional Questions\n",
    "order: 85\n",
    "---"
   ]
  },
  {
   "cell_type": "markdown",
   "metadata": {},
   "source": [
    "## Example 1 (Proof of equality constraint EL Equation)\n",
    "\n",
    "_Consider the problem_\n",
    "\\begin{align*}\n",
    "\\text{minimize}\\quad &I[x(\\cdot)] = \\frac12\\int_0^\\pi [x'(t)]^2 dt\\\\\n",
    "\\text{subject to} \\quad & J[x(\\cdot)] = \\int_0^\\pi [x(t)]^2 dt = 1\\\\\n",
    "\\text{with conditions} \\quad &x\\in \\mathcal A :=\\{x:[0,\\pi]\\rightarrow \\mathbb R\\mid x(0) = x(\\pi) = 0\\}\n",
    "\\end{align*}\n",
    "_Suppose $x$ is a $C^2$ function that solve the problem, let $y\\in \\mathcal A$ be $C^2$, define_\n",
    "$$a(s) = \\bigg[\\int_0^\\pi(x(t) + sy(t))^2 dt\\bigg]^{1/2}$$\n",
    "$$i(s) = I[\\frac{x(\\cdot) + sy(\\cdot))}{a(s)}]$$\n",
    "\n",
    "_(a) Show that $a(0) = 1, i'(0) = 0$_\n",
    "\n",
    "_proof._   \n",
    "$$a(0) = (\\int_0^\\pi (x(t) + 0y(t)^2)dt)^{1/2} = (\\int_0^\\pi x(t)^2dt)^{1/2}$$\n",
    "Since $x$ solve the problem, it must follows the constraint $\\int_0^\\pi x(t) = 1$\n",
    "$$a(0) = (\\int_0^\\pi x(t)^2dt)^{1/2} = 1$$\n",
    "Since $x$ is the minimizer, FONC gives that $$\\frac{d}{ds}\\mid_{s=0}I[x(\\cdot) + sy(\\cdot)] = 0$$\n",
    "for any test function $y\\in\\mathcal A$, note that \n",
    "$$\\frac{d}{ds}\\mid_{s=0}I[x(\\cdot) + sy(\\cdot)] = \\frac{d}{ds}\\mid_{s=0}I[\\frac{x(\\cdot) + sy(\\cdot)}{1}] = i'(0) = 0$$\n",
    "\n",
    "_(b) Show that_\n",
    "$$i'(0) = \\int_0^\\pi x'(t)y'(t)dt - \\lambda \\int_0^\\pi x(t)y(t)dt$$\n",
    "_for constant $\\lambda$ in terms of $x(t)$_\n",
    "\n",
    "_proof_. \n",
    "By multiplication rule\n",
    "$$\n",
    "i'(s) = -2a(s)^{-3}a'(s)I[x + sy] + a(s)^{-2}\\frac{d}{ds}I[x+sy]$$\n",
    "Evaluate at $s=0$ with $a(0) = 1$, we have\n",
    "$$\n",
    "i'(0) = -2a'(0)I[x(\\cdot)] + \\left.\\frac{d}{ds}\\right\\vert_{s=0}I[x(\\cdot) + sy(\\cdot)]\n",
    "$$\n",
    "Then, note that \n",
    "\\begin{align*}\n",
    "a'(s) &= \\frac{1}{2}\\bigg(\\int_0^\\pi(x(t) + sy(t))^2 dt\\bigg)^{-1/2}\\\\&\\quad\\frac{d}{ds}\\int_0^\\pi(x(t) + sy(t))^2dt\\\\\n",
    "&= \\frac{1}{2}a(s)^{-1} 2\\int_0^\\pi (x(t) + sy(t))y(t)dt &\\text{Leibniz rule}\\\\\n",
    "a'(0) &= \\int_0^\\pi(x(t)+0y(t))y(t)dt \\\\\n",
    "&= \\int_0^\\pi x(t)y(t)dt\\\\\n",
    "\\frac{d}{ds}I[x + sy]&= \\frac{1}{2}\\frac{d}{ds}\\int_0^\\pi(\\frac d{dt} x(t)+sy(t))^2 dt\\\\\n",
    "&= \\frac12\\frac{d}{ds}\\int_0^\\pi (x'(t) + sy'(t))^2dt\\\\\n",
    "&= \\frac12\\int_0^\\pi \\frac{d}{ds}(x'(t) + sy'(t))^2dt&\\text{Leibniz rule}\\\\\n",
    "&= \\int_0^\\pi (x'(t)+sy'(t))y'(t)dt\\\\\n",
    "\\left.\\frac{d}{ds}\\right\\vert_{s=0}I[x(\\cdot) + sy(\\cdot)]&= \\int_0^\\pi(x'(t) + 0 y'(t))y'(t)dt \\\\\n",
    "&= \\int_0^\\pi x'(t)y'(t)dt\\\\\n",
    "i'(0) &= -2I[x(\\cdot)]\\int_0^\\pi x(t)y(t)dt + \\int_0^\\pi x'(t)y'(t)dt\n",
    "\\end{align*}\n",
    "so that let $\\lambda = -2 I[x(\\cdot)]$ we have \n",
    "$$i'(0) = \\int_0^\\pi x'(t)y'(t)dt -\\lambda \\int_0^\\pi x(t)y(t)dt$$\n",
    "\n",
    "_(c) Show that $x''(t) + \\lambda x(t) = 0$ for $0 <t<\\pi$_\n",
    "\n",
    "_proof_. Note that $i'(0) = 0$\n",
    "so that \n",
    "\\begin{align*}\n",
    "0 &= \\int_0^\\pi x'(t)y'(t)dt -\\lambda \\int_0^\\pi x(t)y(t)dt\\\\\n",
    "&= x'(t)y(t)\\vert^\\pi_0 - \\int_0^\\pi x''(t)y(t)dt -\\lambda\\int_0^\\pi x(t)y(t)dt&\\text{integration by parts}\\\\\n",
    "&= 0 - \\int_0^\\pi x''(t)y(t) + \\lambda x(t)y(t)dt\\\\\n",
    "0 &= \\int_0^\\pi (x''(t) + \\lambda x(t))y(t)dt\n",
    "\\end{align*}\n",
    "To satisfy this equation for all $y\\in\\mathcal A$, we must have $x''(t) + \\lambda x(t) = 0$\n",
    "\n",
    "## Example 2\n",
    "_Let $\\mathcal A = \\{u:[0,1]\\rightarrow\\mathbb R^3\\mid u\\in C^1 u(0)=A, u(1)=B\\}$, consider the \"holonomic constraints\" problem\n",
    "\\begin{align*}\n",
    "\\text{minimize}\\quad F[u(\\cdot)]:=\\int_0^1 \\sqrt{u'_1(t)^2 + u'_2(t)^2 + u'_3(t)^2}dt\\\\\n",
    "\\text{subject to}\\quad u\\in\\mathcal A, G(u(t)) = u_1(t)^2 + u_2(t)^2 = 1\n",
    "\\end{align*}\n",
    "Find EL equations for this problem_\n",
    "\n",
    "\\begin{align*}\n",
    "L(t, z_1,z_2,z_3,p_1,p_2,p_3) &= (p_1^2 + p_2^2+p_3^2)^{1/2}\\\\\n",
    "L_z &= 0\\\\\n",
    "L_{p_i} &= p_i(p_1^2 + p_2^2+p_3^2)^{-1/2} \\\\\n",
    "&= \\frac{u'_i(t)}{\\sqrt{u'_1(t)^2 + u'_2(t)^2 + u'_3(t)^2}}\\\\\n",
    "\\nabla_u G &= (2u_1(t), 2u_2(t), 0)\\\\\n",
    "\\frac{\\partial F}{\\partial u_1} &= 0 - \\frac{d}{dt}L_{p_i}\\\\\n",
    "&= -\\frac{d}{dt} \\frac{u'_i(t)}{\\sqrt{u'_1(t)^2 + u'_2(t)^2 + u'_3(t)^2}}\n",
    "\\end{align*}\n",
    "Therefore, for some $\\lambda:[0, 1]\\rightarrow \\mathbb R$, the EL equations is \n",
    "$$\\begin{bmatrix}\n",
    "-\\frac{d}{dt} \\frac{u'_1(t)}{\\sqrt{u'_1(t)^2 + u'_2(t)^2 + u'_3(t)^2}}\\\\\n",
    "-\\frac{d}{dt} \\frac{u'_2(t)}{\\sqrt{u'_1(t)^2 + u'_2(t)^2 + u'_3(t)^2}}\\\\\n",
    "-\\frac{d}{dt} \\frac{u'_3(t)}{\\sqrt{u'_1(t)^2 + u'_2(t)^2 + u'_3(t)^2}}\n",
    "\\end{bmatrix} + \\lambda(t)\n",
    "\\begin{bmatrix}\n",
    "2u_1(t)\\\\\n",
    "2u_2(t)\\\\\n",
    "0\n",
    "\\end{bmatrix} =\\begin{bmatrix}\n",
    "0\\\\0\\\\0\n",
    "\\end{bmatrix} $$\n",
    "\n",
    "## Example 3\n",
    "\n",
    "_Let $\\mathcal A = \\{u:[0,1]\\rightarrow\\mathbb R^2\\mid u\\in C^1, u(0)=A, u(1)=B\\}$, consider the \"holonomic constraints\" problem_\n",
    "\\begin{align*}\n",
    "\\text{minimize}\\quad F[u(\\cdot)]:=\\int_0^1 \\sqrt{u'_1(t)^2 + u'_2(t)^2}dt\\\\\n",
    "\\text{subject to}\\quad u\\in\\mathcal A, G(u(t)) = u_1(t) + u_2(t)^2 = 1\n",
    "\\end{align*}\n",
    "\n",
    "_(a) Find the EL Equation_\n",
    "\n",
    "We can easily have the EL equations being\n",
    "$$\\begin{bmatrix}\n",
    "-\\frac{d}{dt} \\frac{u'_1(t)}{\\sqrt{u'_1(t)^2 + u'_2(t)^2}}\\\\\n",
    "-\\frac{d}{dt} \\frac{u'_2(t)}{\\sqrt{u'_1(t)^2 + u'_2(t)^2}}\n",
    "\\end{bmatrix} + \\lambda(t)\n",
    "\\begin{bmatrix}\n",
    "1\\\\\n",
    "2u_2(t)\n",
    "\\end{bmatrix} =\\begin{bmatrix}\n",
    "0\\\\0\n",
    "\\end{bmatrix} $$\n",
    "\n",
    "_(b) Solve the problem as a unconstrainted problem_\n",
    "\n",
    "Consider $u_2\\in \\{v:[0, 1]\\rightarrow \\mathbb R\\mid v(0) = a, v(1) = b, v\\in C^1\\}$, the original problem is equivalent to minimize \n",
    "\\begin{align*}\n",
    "F[v(\\cdot)] &= \\int_0^1 \\sqrt{u_2'(t)^2 + \\big[\\frac{d}{dt}(1-u_2(t)^2)\\big]^2}dt\\\\\n",
    "&= \\int_0^1 \\sqrt{u_2'(t)^2 + (-2u_2(t)u_2'(t))^2}\\\\\n",
    "&= \\int_0^1 \\sqrt{(1 + 4u_2(t)^2)u_2'(t)^2}dt\\\\\n",
    "L(x, z, p) &= \\sqrt{(1+4z^2)p^2}\\\\\n",
    "L_z &= ((1+4z^2)p^2)^{-1/2}(4p^2z)\\\\\n",
    "&= \\frac{4u_2(t)u_2'(t)^2}{\\sqrt{u_2'(t)^2 + \\big[\\frac{d}{dt}(1-u_2(t)^2)\\big]^2}}\\\\\n",
    "L_p &= ((1+4z^2)p^2)^{-1/2}(1+4z^2)p\\\\\n",
    "\\frac{d}{dt}L_p &= \\frac{d}{dt}\\frac{(1 + 4u_2(t)^2)u_2'(t)}{\\sqrt{u_2'(t)^2 + \\big[\\frac{d}{dt}(1-u_2(t)^2)\\big]^2}}\n",
    "\\end{align*}\n",
    "so that the EL equations give \n",
    "$$- \\frac{d}{dt}\\frac{(1 + 4u_2(t)^2)u_2'(t)}{\\sqrt{u_2'(t)^2 + \\big[\\frac{d}{dt}(1-u_2(t)^2)\\big]^2}} + \\frac{4u_2(t)u_2'(t)^2}{\\sqrt{u_2'(t)^2 + \\big[\\frac{d}{dt}(1-u_2(t)^2)\\big]^2}}= 0 $$\n",
    "\n",
    "_(c) Show that (a) and (b) gives the same answer_\n",
    "\n",
    "From (a), we have \n",
    "$$\\lambda(t) = \\frac{d}{dt}\\frac{u'_1(t)}{\\sqrt{u'_1(t)^2 + u'_2(t)^2}}$$\n",
    "From (b), note that $u_1' = \\frac{d}{dt}(1-u_2^2) = -2u_2u_2'$\n",
    "so that we can write\n",
    "\\begin{align*}\n",
    "- \\frac{d}{dt}\\frac{(1 + 4u_2(t)^2)u_2'(t)}{\\sqrt{u_2'(t)^2 + \\big[\\frac{d}{dt}(1-u_2(t)^2)\\big]^2}} + \\frac{4u_2(t)u_2'(t)^2}{\\sqrt{u_2'(t)^2 + \\big[\\frac{d}{dt}(1-u_2(t)^2)\\big]^2}}&= 0 \\\\\n",
    "-\\frac{d}{dt}\\frac{u_2'}{\\sqrt{u_1'(t)^2 + u_2'(t)^2}} + \\frac{d}{dt}\\frac{2u_2(t)u_1'(t)}{{\\sqrt{u_1'(t)^2 + u_2'(t)^2}}} + \\frac{2u_2'(t)u_1'(t)}{{\\sqrt{u_1'(t)^2 + u_2'(t)^2}}}&=0\\\\\n",
    "-\\frac{d}{dt}\\frac{u_2'}{\\sqrt{u_1'(t)^2 + u_2'(t)^2}} + 2u_2(t)\\frac{d}{dt}\\frac{u_1'(t)}{{\\sqrt{u_1'(t)^2 + u_2'(t)^2}}} &= 0\\\\\n",
    "-\\frac{d}{dt}\\frac{u_2'}{\\sqrt{u_1'(t)^2 + u_2'(t)^2}} + 2u_2(t)\\lambda(t) &= 0\\\\\n",
    "\\end{align*}\n",
    "\n",
    "## Example 4\n",
    "\n",
    "_Let $u\\in \\mathcal A = \\{u:[0, 1]\\rightarrow \\mathbb R\\mid u\\in C^1, u(0) = 0\\}$_\n",
    "\\begin{align*}\\text{minimize}\\quad &F[u] = \\int_0^1L^F(x, u(x), u'(x))dx\\\\\n",
    "\\text{subject to}\\quad &G[u] =\\int_0^1 u'(x)dx = a\n",
    "\\end{align*}\n",
    "\n",
    "_(a) Write the EL Equation_\n",
    "\n",
    "\\begin{align*}\n",
    "\\frac{\\partial F}{\\partial u} &= L^F_z(x, u(x), u'(x)) - \\frac{d}{dx}L^F_p(x, u(x), u'(x))\\\\\n",
    "L^G(x, z, p) &= p\\\\\n",
    "\\frac{d}{dt}L^G_p &= \\frac{d}{dt}1 = 0\\\\\n",
    "\\frac{\\partial G}{\\partial u} &= 0\n",
    "\\end{align*}\n",
    "$$L^F_z(x, u(x), u'(x)) - \\frac{d}{dx}L^F_p(x, u(x), u'(x)) - \\lambda\\times 0= 0$$\n",
    "And $G[u] = \\int_0^1 u'(x)dx = u(x)\\mid^1_0 = u(1) - 0 = a$, note that this constraint makes the two end points of $u$ fixed, so EL equation is the only needed first order necessary condition.  \n",
    "So that we have \n",
    "$$L^F_z(x, u(x), u'(x)) - \\frac{d}{dx}L^F_p(x, u(x), u'(x))= 0$$\n",
    "$$u(1) = a$$\n",
    "\n",
    "_(b) Formulated the problem as a unconstrianed problem and solve it_\n",
    "\n",
    "Note that $G[u] = u(1) - u(0) = u(1) = a$ so that the problem is to minimize $F[u]$ on $u\\in \\{u:[0, 1]\\rightarrow \\mathbb R\\mid u\\in C^1, u(0) = 0, u(1) =a\\}$, hence the EL equation is simply \n",
    "$$L^F_z(x, u(x), u'(x)) - \\frac{d}{dx}L^F_p(x, u(x), u'(x)) = 0$$\n",
    "\n",
    "_(c) Show (a) and (b) gives the same answer_\n",
    "\n",
    "Trivially, \n",
    "$$L^F_z(x, u(x), u'(x)) - \\frac{d}{dx}L^F_p(x, u(x), u'(x))= 0$$\n",
    "$$u(1) = a$$\n",
    "$$u\\in \\{u:[0, 1]\\rightarrow \\mathbb R\\mid u\\in C^1, u(0) = 0\\}$$\n",
    "Is the same as \n",
    "$$L^F_z(x, u(x), u'(x)) - \\frac{d}{dx}L^F_p(x, u(x), u'(x))= 0$$\n",
    "$$u\\in \\{u:[0, 1]\\rightarrow \\mathbb R\\mid u\\in C^1, u(0) = 0, u(1) = a\\}$$\n",
    "\n",
    "## Example 5\n",
    "\n",
    "_Consider the minimization problem in Q4, but the two endpoints are both unfixed, find the FONC_\n",
    "\n",
    "Note that the constraint $G[u] = \\int_0^1 u'(x)dx = u(1) - u(0) = a$, so that we are optimize $F[u]$ on $\\mathcal A := \\{u[0, 1]\\rightarrow \\mathbb R\\mid u\\in C^1, u(1)-u(0) = a\\}$.  \n",
    "Consider test function $v$ s.t. $v(0) = v(1) = 0$.  \n",
    "Assume $u_*$ is a minimizer, define \n",
    "$$f(s, t):\\mathbb R^2\\rightarrow \\mathbb R := F[u_*(\\cdot) + sv(\\cdot) + t] = \\int_0^1 L(x, u(x)+sv(x)+t, u'(x) + sv'(x))dx$$\n",
    "so that $$\\mathcal A = \\{u_*+sv+t\\mid s,t\\in\\mathbb R\\}$$\n",
    "Since $u_*$ is a minimizer, we must have $\\nabla f = 0$\n",
    "$$\\frac{\\partial}{\\partial s}\\mid_{(s,t)=(0, 0)}F = \\int_0^1 L_z^F(\\cdots)v(x) + L_p^G(\\cdots)v'(x)dx = \\int_0^1(L_z - \\frac{d}{dx}L_p)v(x)dx$$\n",
    "The computation of the above equation is identical to the proof of Euler Lagrange equation, and by fundamental lemma, we have must \n",
    "$$L_z(x, u(x), u'(x)) - \\frac{d}{dx}L_p(x, u(x), u'(x)) = 0$$\n",
    "Then, we also need to have\n",
    "$$\\frac{\\partial}{\\partial t}\\mid_{(s,t) =(0,0)}F = \\int_0^1 L_z^F(x, u(x), u'(x)) dx=0$$\n",
    "so that FONC are \n",
    "$$L_z(x, u(x), u'(x)) - \\frac{d}{dx}L_p(x, u(x), u'(x)) = 0$$\n",
    "$$\\int_0^1 L_z^F(x, u(x), u'(x)) dx=0$$\n",
    "\n",
    "## Example 6\n",
    "_Prove Euler-Lagrange equation for isoperimetric problems_\n",
    "\n",
    "_proof_. Take $v_2$ s.t. $\\int_a^b \\frac{\\partial G}{\\partial u}(u_*)(x)v_2(x)dx \\neq 0$. Let $f(s, t) = F[u_* +sv_1 + tv_2]$ and $g(s, t) = G[u_*+sv_1+tv_2]$. \n",
    "Note that \n",
    "\\begin{align*}\n",
    "\\frac{\\partial}{\\partial s}g(0, 0) &= \\int_a^b \\frac{\\partial}{\\partial s}\\mid_{(s, t)=(0, 0)}L^G(x, u_* + sv_1 + tv_2, u_*'+sv_1'+tv_2')dx\\\\\n",
    "&= \\int_a^b L_z^G(\\cdots)\\frac{\\partial}{\\partial s}(u_*+sv_1+tv_2) + L_p^G(\\cdots)\\frac{\\partial}{\\partial s}(u_*'+sv_1'+tv_2')\\\\\n",
    "&= \\int_a^b L_z^G(\\cdots)v_1(x) + L_p^G(\\cdots)v_1'(x)\\\\\n",
    "&=\\int_a^b (L_z^G(x, u_*, u_*') - \\frac{d}{dx}L_p^G(x, u_*, u_*'))v_1(x)dx\\\\\n",
    "&= \\int_{a}^b \\frac{\\partial G}{\\partial u}(u_*)(x)v_1(x)dx\n",
    "\\end{align*}\n",
    "The above equation is obtained by integration by parts, the steps are identical to the computation for $\\frac{d}{ds}\\mid_{s=0}F[u+sv]$.  \n",
    "With the similar derivations, we can show that \n",
    "$$\\frac{\\partial}{\\partial t}g(0, 0) = \\int_{a}^b \\frac{\\partial G}{\\partial u}(u_*)(x)v_2(x)dx$$\n",
    "$$\\frac{\\partial}{\\partial t}f(0,0) = \\int_{a}^b \\frac{\\partial F}{\\partial u}(u_*)(x)v_1(x)dx$$\n",
    "$$\\frac{\\partial}{\\partial t}f(0,0) = \\int_{a}^b \\frac{\\partial F}{\\partial u}(u_*)(x)v_1(x)dx$$\n",
    "Note that by our assumption, $\\frac{\\partial}{\\partial t}g(0,0) = \\int_{a}^b \\frac{\\partial G}{\\partial u}(u_*)(x)v_2(x)dx\\neq 0$ so that $\\nabla g(0, 0) \\neq 0$, therefore we can safely apply Lagrange multipliers, i.e. for some $\\lambda$\n",
    "\\begin{align*}0 &= \\int_{a}^b \\frac{\\partial F}{\\partial u}(u_*)(x)v_1(x)dx + \\lambda \\int_{a}^b \\frac{\\partial G}{\\partial u}(u_*)(x)v_1(x)dx \\\\\n",
    "&= \\int_a^b (\\frac{\\partial F}{\\partial u} + \\lambda \\frac{\\partial G}{\\partial u})v_1(x)dx\\\\\n",
    "0 &= \\int_{a}^b \\frac{\\partial F}{\\partial u}(u_*)(x)v_2(x)dx + \\lambda \\int_{a}^b \\frac{\\partial G}{\\partial u}(u_*)(x)v_2(x)dx \\\\\n",
    "&= \\int_a^b (\\frac{\\partial F}{\\partial u} + \\lambda \\frac{\\partial G}{\\partial u})v_2(x)dx\\\\\n",
    "\\end{align*}\n",
    "By fundamental lemma, both equations lead to \n",
    "$$\\frac{\\partial F}{\\partial u} + \\lambda \\frac{\\partial G}{\\partial u} = 0$$\n",
    "a.k.a\n",
    "$$L_z^F - \\frac{d}{dx}L_p^F + \\lambda(L_z^G - \\frac{d}{dx}L_p^G) = 0$$\n",
    "$$-\\frac{d}{dx}(L^G+\\lambda L^G)_p(x, u_*, u'_*) + (L^F+\\lambda L^G)_z(x, u_*,u_*') = 0$$"
   ]
  }
 ],
 "metadata": {
  "hide_input": false,
  "kernelspec": {
   "display_name": "Python 3",
   "language": "python",
   "name": "python3"
  },
  "language_info": {
   "codemirror_mode": {
    "name": "ipython",
    "version": 3
   },
   "file_extension": ".py",
   "mimetype": "text/x-python",
   "name": "python",
   "nbconvert_exporter": "python",
   "pygments_lexer": "ipython3",
   "version": "3.7.6"
  }
 },
 "nbformat": 4,
 "nbformat_minor": 4
}
