{
 "cells": [
  {
   "cell_type": "raw",
   "metadata": {},
   "source": [
    "---\n",
    "title: Unconstrainted Optimization on Calulus of Variations Additional Questions\n",
    "order: 75\n",
    "---"
   ]
  },
  {
   "cell_type": "markdown",
   "metadata": {},
   "source": [
    "## Example 1\n",
    "\n",
    "_Consider $Q+scc^T$ where $Q$ is positive definite symmetric, prove that the largest eigenvalue $\\mu_n(s)$ of $Q+scc^T$ is bounded by $a_2 + \\beta s \\leq \\mu_n(s) \\leq a_1 + \\beta s$_\n",
    "\n",
    "_proof_. \n",
    "\\begin{align*}\n",
    "\\mu_n(s) &= \\max_{\\|x\\|=1}\\big\\{x^T(Q+scc^T)x\\big\\}\\\\\n",
    "&= \\max_{\\|x\\|=1} \\big\\{x^TQx + x^Tscc^Tx\\big\\}\n",
    "\\end{align*}\n",
    "Because $Q$ is positive definite, $x^TQx \\geq 0$, \n",
    "\\begin{align*}\n",
    "\\mu_n(s) &\\geq \\max_{\\|x\\|=1} \\big\\{x^Tscc^Tx\\big\\}\\\\\n",
    "&= \\max_{\\|x\\|=1} \\big\\{x^Tcc^Tx\\big\\}s &s\\text{ is a scalar}\n",
    "\\end{align*}\n",
    "Also, we have \n",
    "\\begin{align*}\n",
    "\\mu_n(s) &\\leq \\max_{\\|x\\|=1}\\big\\{x^TQx\\big\\} + \\max_{\\|x\\|=1} \\big\\{x^Tscc^Tx\\big\\}\\\\\n",
    "&= \\max_{\\|x\\|=1}\\big\\{x^TQx\\big\\} + \\max_{\\|x\\|=1} \\big\\{x^Tcc^Tx\\big\\}s\n",
    "\\end{align*}\n",
    "Let $\\alpha_2 = 0, \\alpha_1 = \\max_{\\|x\\|=1}\\big\\{x^TQx\\big\\}, \\beta = \\max_{\\|x\\|=1} \\big\\{x^Tcc^Tx\\big\\}$, since $c\\neq 0, \\beta > 0$. Therefore, \n",
    "$$a_2 + \\beta s \\leq \\mu_n(s) \\leq a_1 + \\beta s$$\n",
    "\n",
    "## Example 2\n",
    "_Derive the formula $p(t):\\mathbb R\\rightarrow \\mathbb R^2 := (x(t), y(t))$ where $p(t)$ is the position of point on the rim of a circle of radius $R$, the circle is rolling along the $x$-axis at a constant speed $a$. Assume $c(t) = (at, R)$ is the position of the center of the circle at $t$ and $p(0) = (0, 0)$._\n",
    "\n",
    "Let $f(\\theta):\\mathbb R\\rightarrow \\mathbb R^2 := (R\\cos\\theta, R\\sin\\theta)$ be the parametric equation of the circle.\n",
    "\n",
    "Consider the point $q(t) = (at, 0)$ on the rim of the circle at time $t$, let \n",
    "$$q_c(t) = q(t) - c(t) = (at, 0) - (at, R) = (0, -R)$$ be its position relative to the center of the circle, note that \n",
    "$$q_c(t) = f(-\\pi/2) = (\\cos(-\\frac{\\pi}{2}), \\sin(-\\frac{\\pi}{2}))$$\n",
    "Then, let $L$ be the arc of the circle between $q_c$ and $p_c$ and $\\theta(t)$ be the angle subtended by arc $L$ from the center of the circle. Since the arc length is $at$, we have\n",
    "\\begin{align*}\n",
    "\\theta(0) - \\theta(t) &= \\frac{at}{R}\\\\\n",
    "\\theta(t) &= \\theta(0) - \\frac{at}{R}\\\\\n",
    "\\theta(t) &= -\\frac{\\pi}{2} - \\frac{at}{R}\n",
    "\\end{align*}\n",
    "Therefore, let $q_c(t)$ be $p$'s position relative to the center of the circle, $$q_c(t) = f(\\theta(t)) = \\big(R\\cos(-\\frac{\\pi}{2} - \\frac{at}{R}), R\\sin(-\\frac{\\pi}{2} - \\frac{at}{R})\\big)$$\n",
    "so that \n",
    "$$p(t) = p_c(t) + c(t) = \\big(at + R\\cos(-\\frac{\\pi}{2} - \\frac{at}{R}), R\\sin(-\\frac{\\pi}{2} - \\frac{at}{R})\\big)$$\n",
    "\n",
    "## Example 3\n",
    "$$F[\\mu[\\cdot] = \\int_a^b L(x, \\mu(x), \\mu'(x))dx, x(a)=A, x(b)=B$$\n",
    "_$L, \\mu \\in C^2$, partition $[a,b]$ into $x_0, ..., x_{n+1}$ where $x_i = a + \\frac{b-a}{n+1}i$ so that we can approximate the functional by_ \n",
    "$$F:\\mathbb R^n\\rightarrow \\mathbb R, F(\\mu_1, ..., \\mu_n) :=\\sum_{i=1}^{n+1}L(x_i, \\mu_i, \\frac{\\mu_i - \\mu_{i-1}}{h})h$$\n",
    "\n",
    "_(a) Calculate $\\frac{dF}{d\\mu_i}(\\mu)$_\n",
    "\\begin{align*}\n",
    "\\frac{dF}{d\\mu_i}(\\mu) &= \\sum_{j=1}^{n+1}\\frac{d}{d\\mu_i}L(x_j, \\mu_j, \\frac{\\mu_j - \\mu_{j-1}}{h})h\\\\\n",
    "&= \\frac{d}{d\\mu_i}L(x_{i}, \\mu_{i}, \\frac{\\mu_i - \\mu_{i-1}}{h})h + \\frac{d}{d\\mu_i}L(x_{i+1}, \\mu_{i+1}, \\frac{\\mu_{i+1} - \\mu_{i}}{h})h\\\\\n",
    "&= L_z(x_{i}, \\mu_{i}, \\frac{\\mu_i - \\mu_{i-1}}{h})h\\frac{d}{d\\mu_i}\\mu_i + L_p(x_{i}, \\mu_{i}, \\frac{\\mu_i - \\mu_{i-1}}{h})h\\frac{d}{d\\mu_i}\\frac{\\mu_i - \\mu_{i-1}}{h}\\\\\n",
    "&\\quad+L_p(x_{i+1}, \\mu_{i+1}, \\frac{\\mu_{i+1} - \\mu_{i}}{h})h\\frac{d}{d\\mu_i}\\frac{\\mu_{i+1} - \\mu_{i}}{h}\\\\\n",
    "&= hL_z(x_{i}, \\mu_{i}, \\frac{\\mu_i - \\mu_{i-1}}{h}) - (L_p(x_{i+1}, \\mu_{i+1}, \\frac{\\mu_{i+1} - \\mu_{i}}{h})- L_p(x_{i}, \\mu_{i}, \\frac{\\mu_i - \\mu_{i-1}}{h}))\n",
    "\\end{align*}\n",
    "\n",
    "_(b) Take $h\\rightarrow 0$, show that $\\frac{dF}{d\\mu_i}(\\mu) = 0\\Rightarrow L_z(x, \\mu(x), \\mu'(x) - \\frac{d}{dx}L_p(x, \\mu(x), \\mu'(x))) = 0$_\n",
    "\n",
    "_proof_. Since $\\frac{dF}{d\\mu_i}(\\mu) = 0$\n",
    "\\begin{align*}\n",
    "\\lim_{h\\rightarrow 0} \\frac{1}{h}\\frac{dF}{d\\mu_i}(\\mu) &= \\lim_{h\\rightarrow 0}L_z(x_i, \\mu_i, \\frac{\\mu_i-\\mu_{i-1}}h) \\\\\n",
    "&\\quad- \\lim_{h\\rightarrow 0}\\frac{L_p(x_{i+1}, \\mu_{i+1}, \\frac{\\mu_{i+1} - \\mu_{i}}{h})- L_p(x_{i}, \\mu_{i}, \\frac{\\mu_i - \\mu_{i-1}}{h})}{h}\\\\\n",
    "&= L_z(x_i, \\mu(x_i), \\mu(x_i)')\\\\\n",
    "&\\quad - \\lim_{h\\rightarrow 0}\\frac{L_p(x_i+h, \\mu(x_i+h), \\mu'(x_i+h))- L_p(x_{i}, \\mu(x_i), \\mu'(x_i))}{h}\\\\\n",
    "&\\text{by definition of derivative}\\\\\n",
    "&= L_z(x_i, \\mu(x_i), \\mu(x_i)') - \\frac{d}{dx}L_p(x_i, \\mu(x_i), \\mu(x_i)')\n",
    "\\end{align*}\n",
    "Therefore, for some $x\\in[a,b]$, since $h\\rightarrow 0$, we can partition $[a,b]$ s.t. $x\\in \\text{partition}(a, b)$, so that we have \n",
    "$$L_z(x_i, \\mu(x_i), \\mu(x_i)') - \\frac{d}{dx}L_p(x_i, \\mu(x_i), \\mu(x_i)') = \\lim_{h\\rightarrow 0} \\frac{1}{h}\\frac{dF}{d\\mu_i}(\\mu) = 0$$\n",
    "\n",
    "\n",
    "\n",
    "## Example 4\n",
    "\n",
    "_Find FONC of_\n",
    "\\begin{align*}\n",
    "\\text{minimize}\\quad &F[\\mu(\\cdot)] := \\int_a^b L(x, u(x), u'(x))dx\\\\\n",
    "\\text{subject to}\\quad &\\mu\\in \\mathcal A:= \\{\\mu:[a,b]\\rightarrow\\mathbb R\\mid \\mu\\in C^2, \\mu(a) = A\\}\n",
    "\\end{align*}\n",
    "\n",
    "Let $\\mu_*$ be the minimizer of the problem.  \n",
    "Let $\\mathcal T:= \\{v:[a, b]\\rightarrow\\mathbb R\\mid v\\in C^2, v(a) = 0\\}$ be the set of test functions so that $\\forall v\\in \\mathcal T. \\forall s\\in\\mathbb R. u_*+sv \\in \\mathcal A$.  \n",
    "Then as what have been done in the class till the integrations by parts \n",
    "\\begin{align*}\n",
    "\\frac{d}{ds}F[u_*+sv]\n",
    "&=\\int_a^b \\big[L_z(...) - \\frac{d}{dx}L_p(...)\\big]v(x)dx + \\big[L_p(...)\\mid_a^b\\big]\n",
    "\\end{align*}\n",
    "Since $v(a) = 0$, note that \n",
    "\\begin{align*}\n",
    "\\big[L_p(x, u_*(x), u_*'(x))v(x)\\mid_a^b\\big] &= L_p(b, u_*(b), u_*'(b))v(b) - L_p(a, u_*(a), u_*'(a))v(a)\\\\\n",
    "&= L_p(b, u_*(b), u_*'(b))v(b)\n",
    "\\end{align*}\n",
    "Consider $v_1\\in\\mathcal T$ s.t. $v(b) = 0$, hence  \n",
    "$$\\big[L_p(x, u_*(x), u_*'(x))v(x)\\mid_a^b\\big] = 0$$ \n",
    "Given $u_*$ is the minimizer,  \n",
    "$$0 = \\frac{d}{ds}F[u_*+sv] =\\int_a^b \\big[L_z(...) - \\frac{d}{dx}L_p(...)\\big]v(x)dx$$\n",
    "follows the original Euler-Lagrange equation, i.e. \n",
    "$$L_z(x, u_*(x), u_*'(x)) - \\frac{d}{dx}L_p(x, u_*(x), u_*'(x)) = 0$$\n",
    "Consider $v_2\\in\\mathcal T, v_2(b)\\neq 0$, since we have to fulfill the necessary conditions for cases like $v_1$, we have \n",
    "$$L_z(x, u(x), u'(x)) - \\frac{d}{dx}L_p(x, u(x), u'(x)) = 0$$\n",
    "so that \n",
    "$$0 = \\frac{d}{ds}F[u_*+sv] = 0 + L_p(b, u(b), u'(b))v(b)$$\n",
    "Therefore, there are two FONC as\n",
    "$$L_z(x, u_*(x), u_*'(x)) - \\frac{d}{dx}L_p(x, u_*(x), u_*'(x)) = 0$$\n",
    "$$L_p(b, u(b), u'(b))v(b) = 0$$\n"
   ]
  }
 ],
 "metadata": {
  "hide_input": false,
  "kernelspec": {
   "display_name": "Python 3",
   "language": "python",
   "name": "python3"
  },
  "language_info": {
   "codemirror_mode": {
    "name": "ipython",
    "version": 3
   },
   "file_extension": ".py",
   "mimetype": "text/x-python",
   "name": "python",
   "nbconvert_exporter": "python",
   "pygments_lexer": "ipython3",
   "version": "3.7.6"
  }
 },
 "nbformat": 4,
 "nbformat_minor": 4
}
